Restore the weaker notion of atomicity (both are now available).

theories/program_logic/language.v
@@ -34,7 +34,11 @@ Section language.
 
   Definition reducible (e : expr Λ) (σ : state Λ) :=
     ∃ e' σ' efs, prim_step e σ e' σ' efs.
+  Definition irreducible (e : expr Λ) (σ : state Λ) :=
+    ∀e' σ' efs, ¬prim_step e σ e' σ' efs. 
   Definition atomic (e : expr Λ) : Prop :=
+    ∀ σ e' σ' efs, prim_step e σ e' σ' efs → irreducible e' σ'.
+  Definition strong_atomic (e : expr Λ) : Prop :=
     ∀ σ e' σ' efs, prim_step e σ e' σ' efs → is_Some (to_val e').
   Definition progress (e : expr Λ) (σ : state Λ) :=
     is_Some (to_val e) ∨ reducible e σ.
@@ -49,6 +53,10 @@ Section language.
   Proof. intros <-. by rewrite to_of_val. Qed.
   Lemma reducible_not_val e σ : reducible e σ → to_val e = None.
   Proof. intros (?&?&?&?); eauto using val_stuck. Qed.
+  Lemma val_irreducible e σ : is_Some (to_val e) → irreducible e σ.
+  Proof. intros [??] ??? ?%val_stuck. by destruct (to_val e). Qed.
+  Lemma weaken_atomic e : strong_atomic e → atomic e.
+  Proof. by intros Ha ???? ?%Ha; apply val_irreducible. Qed.
   Global Instance of_val_inj : Inj (=) (=) (@of_val Λ).
   Proof. by intros v v' Hv; apply (inj Some); rewrite -!to_of_val Hv. Qed.
 End language.
